Collapse unrep definition

Semantics/TreeToGraph.thy
@@ -408,6 +408,18 @@ export_code get_fresh_id
 value "get_fresh_id eg2_sq"
 value "get_fresh_id (add_node 6 (ParameterNode 2, default_stamp) eg2_sq)"
 
+inductive unique :: "IRGraph \<Rightarrow> (IRNode \<times> Stamp) \<Rightarrow> (IRGraph \<times> ID) \<Rightarrow> bool" where
+  Exists:
+  "\<lbrakk>find_node_and_stamp g node = Some n\<rbrakk>
+   \<Longrightarrow> unique g node (g, n)" |
+  New:
+  "\<lbrakk>find_node_and_stamp g node = None;
+    n = get_fresh_id g;
+    g' = add_node n node g\<rbrakk>
+   \<Longrightarrow> unique g node (g', n)"
+
+code_pred (modes: i \<Rightarrow> i \<Rightarrow> o \<Rightarrow> bool as uniqueE) unique .
+
 (* Second version of tree insertion into graph:
 
       g \<triangleleft> expr \<leadsto> (g',n) re-inserts expr into g and returns the new root n.
@@ -416,75 +428,36 @@ value "get_fresh_id (add_node 6 (ParameterNode 2, default_stamp) eg2_sq)"
 *)
 inductive
   unrep :: "IRGraph \<Rightarrow> IRExpr \<Rightarrow> (IRGraph \<times> ID) \<Rightarrow> bool" ("_ \<oplus> _ \<leadsto> _" 55)
-   where
+  where
 
-  ConstantNodeSame:
-  "\<lbrakk>find_node_and_stamp g (ConstantNode c, constantAsStamp c) = Some n\<rbrakk>
-    \<Longrightarrow> g \<oplus> (ConstantExpr c) \<leadsto> (g, n)" |
+  UnrepConstantNode:
+  "\<lbrakk>unique g (ConstantNode c, constantAsStamp c) (g\<^sub>1, n)\<rbrakk>
+    \<Longrightarrow> g \<oplus> (ConstantExpr c) \<leadsto> (g\<^sub>1, n)" |
 
-  ConstantNodeNew:
-  "\<lbrakk>find_node_and_stamp g (ConstantNode c, constantAsStamp c) = None;
-    n = get_fresh_id g;
-    g' = add_node n (ConstantNode c, constantAsStamp c) g \<rbrakk>
-    \<Longrightarrow> g \<oplus> (ConstantExpr c) \<leadsto> (g', n)" |
+  UnrepParameterNode:
+  "\<lbrakk>unique g (ParameterNode i, s) (g\<^sub>1, n)\<rbrakk>
+    \<Longrightarrow> g \<oplus> (ParameterExpr i s) \<leadsto> (g\<^sub>1, n)" |
 
-  ParameterNodeSame:
-  "\<lbrakk>find_node_and_stamp g (ParameterNode i, s) = Some n\<rbrakk>
-    \<Longrightarrow> g \<oplus> (ParameterExpr i s) \<leadsto> (g, n)" |
+  UnrepConditionalNode:
+  "\<lbrakk>g \<oplus> ce \<leadsto> (g\<^sub>1, c);
+    g\<^sub>1 \<oplus> te \<leadsto> (g\<^sub>2, t);
+    g\<^sub>2 \<oplus> fe \<leadsto> (g\<^sub>3, f);
+    s' = meet (stamp g\<^sub>3 t) (stamp g\<^sub>3 f);
+    unique g\<^sub>3 (ConditionalNode c t f, s') (g\<^sub>4, n)\<rbrakk>
+    \<Longrightarrow> g \<oplus> (ConditionalExpr ce te fe) \<leadsto> (g\<^sub>4, n)" |
 
-  ParameterNodeNew:
-  "\<lbrakk>find_node_and_stamp g (ParameterNode i, s) = None;
-    n = get_fresh_id g;
-    g' = add_node n (ParameterNode i, s) g\<rbrakk>
-    \<Longrightarrow> g \<oplus> (ParameterExpr i s) \<leadsto> (g', n)" |
+  UnrepUnaryNode:
+  "\<lbrakk>g \<oplus> xe \<leadsto> (g\<^sub>1, x);
+    s' = stamp_unary op (stamp g\<^sub>1 x);
+    unique g\<^sub>1 (unary_node op x, s') (g\<^sub>2, n)\<rbrakk>
+    \<Longrightarrow> g \<oplus> (UnaryExpr op xe) \<leadsto> (g\<^sub>2, n)" |
 
-  ConditionalNodeSame:
-  "\<lbrakk>find_node_and_stamp g4 (ConditionalNode c t f, s') = Some n;
-    g \<oplus> ce \<leadsto> (g2, c);
-    g2 \<oplus> te \<leadsto> (g3, t);
-    g3 \<oplus> fe \<leadsto> (g4, f);
-    s' = meet (stamp g4 t) (stamp g4 f)\<rbrakk>
-    \<Longrightarrow> g \<oplus> (ConditionalExpr ce te fe) \<leadsto> (g4, n)" |
-
-  ConditionalNodeNew:
-  "\<lbrakk>find_node_and_stamp g4 (ConditionalNode c t f, s') = None;
-    g \<oplus> ce \<leadsto> (g2, c);
-    g2 \<oplus> te \<leadsto> (g3, t);
-    g3 \<oplus> fe \<leadsto> (g4, f);
-    s' = meet (stamp g4 t) (stamp g4 f);
-    n = get_fresh_id g4;
-    g' = add_node n (ConditionalNode c t f, s') g4\<rbrakk>
-    \<Longrightarrow> g \<oplus> (ConditionalExpr ce te fe) \<leadsto> (g', n)" |
-
-  UnaryNodeSame:
-  "\<lbrakk>find_node_and_stamp g' (unary_node op x, s') = Some n;
-    g \<oplus> xe \<leadsto> (g', x);
-    s' = stamp_unary op (stamp g' x)\<rbrakk>
-    \<Longrightarrow> g \<oplus> (UnaryExpr op xe) \<leadsto> (g', n)" |
-
-  UnaryNodeNew:
-  "\<lbrakk>find_node_and_stamp g' (unary_node op x, s') = None;
-    g \<oplus> xe \<leadsto> (g', x);
-    s' = stamp_unary op (stamp g' x);
-    n = get_fresh_id g';
-    g'' = add_node n (unary_node op x, s') g'\<rbrakk>
-    \<Longrightarrow> g \<oplus> (UnaryExpr op xe) \<leadsto> (g'', n)" |
-
-  BinaryNodeSame:
-  "\<lbrakk>find_node_and_stamp g3 (bin_node op x y, s') = Some n;
-    g \<oplus> xe \<leadsto> (g2, x);
-    g2 \<oplus> ye \<leadsto> (g3, y);
-    s' = stamp_binary op (stamp g3 x) (stamp g3 y)\<rbrakk>
-    \<Longrightarrow> g \<oplus> (BinaryExpr op xe ye) \<leadsto> (g3, n)" |
-
-  BinaryNodeNew:
-  "\<lbrakk>find_node_and_stamp g3 (bin_node op x y, s') = None;
-    g \<oplus> xe \<leadsto> (g2, x);
-    g2 \<oplus> ye \<leadsto> (g3, y);
-    s' = stamp_binary op (stamp g3 x) (stamp g3 y);
-    n = get_fresh_id g3;
-    g' = add_node n (bin_node op x y, s') g3\<rbrakk>
-    \<Longrightarrow> g \<oplus> (BinaryExpr op xe ye) \<leadsto> (g', n)" |
+  UnrepBinaryNode:
+  "\<lbrakk>g \<oplus> xe \<leadsto> (g\<^sub>1, x);
+    g\<^sub>1 \<oplus> ye \<leadsto> (g\<^sub>2, y);
+    s' = stamp_binary op (stamp g\<^sub>2 x) (stamp g\<^sub>2 y);
+    unique g\<^sub>2 (bin_node op x y, s') (g\<^sub>3, n)\<rbrakk>
+    \<Longrightarrow> g \<oplus> (BinaryExpr op xe ye) \<leadsto> (g\<^sub>3, n)" |
 
   AllLeafNodes:
   "\<lbrakk>stamp g n = s;
@@ -507,18 +480,20 @@ code_pred (modes: i \<Rightarrow> i \<Rightarrow> o \<Rightarrow> bool as unrepE
   [show_steps,show_mode_inference,show_intermediate_results] 
 *)  unrep .
 
+text_raw \<open>\Snip{unique}%
+\begin{center}
+@{thm[mode=Rule] unique.Exists [no_vars]}\\[8px]
+@{thm[mode=Rule] unique.New [no_vars]}\\[8px]
+\end{center}
+\EndSnip\<close>
+
 text_raw \<open>\Snip{unrepRules}%
 \begin{center}
-@{thm[mode=Rule] unrep.ConstantNodeSame [no_vars]}\\[8px]
-@{thm[mode=Rule] unrep.ConstantNodeNew [no_vars]}\\[8px]
-@{thm[mode=Rule] unrep.ParameterNodeSame [no_vars]}\\[8px]
-@{thm[mode=Rule] unrep.ParameterNodeNew [no_vars]}\\[8px]
-@{thm[mode=Rule] unrep.ConditionalNodeSame [no_vars]}\\[8px]
-@{thm[mode=Rule] unrep.ConditionalNodeNew [no_vars]}\\[8px]
-@{thm[mode=Rule] unrep.BinaryNodeSame [no_vars]}\\[8px]
-@{thm[mode=Rule] unrep.BinaryNodeNew [no_vars]}\\[8px]
-@{thm[mode=Rule] unrep.UnaryNodeSame [no_vars]}\\[8px]
-@{thm[mode=Rule] unrep.UnaryNodeNew [no_vars]}\\[8px]
+@{thm[mode=Rule] unrep.UnrepConstantNode [no_vars]}\\[8px]
+@{thm[mode=Rule] unrep.UnrepParameterNode [no_vars]}\\[8px]
+@{thm[mode=Rule] unrep.UnrepConditionalNode [no_vars]}\\[8px]
+@{thm[mode=Rule] unrep.UnrepBinaryNode [no_vars]}\\[8px]
+@{thm[mode=Rule] unrep.UnrepUnaryNode [no_vars]}\\[8px]
 @{thm[mode=Rule] unrep.AllLeafNodes [no_vars]}\\[8px]
 \end{center}
 \EndSnip\<close>
